compiler/src/compiler/FlatToRiscvLiterals.v
@@ -16,8 +16,8 @@ Require Import coqutil.Tactics.autoforward.
 Import Utility.
 
 Section FlatToRiscvLiterals.
-  Context {p: FlatToRiscv.parameters}.
-  Context {h: FlatToRiscv.assumptions}.
+  Context {p: FlatToRiscvCommon.parameters}.
+  Context {h: FlatToRiscvCommon.assumptions}.
 
   Add Ring wring : (word.ring_theory (word := word))
       (preprocess [autorewrite with rew_word_morphism],
